Rough (backward) proofs of first two AddPhase optimizations plus several typing lemmas for int Values

Optimizations/Canonicalizations/AddPhase.thy
@@ -1,7 +1,59 @@
 theory AddPhase
   imports
     Common
+    Semantics.IRTreeEvalThms
 begin
+
+section \<open>Typing Properties for Integer Values\<close>
+
+text \<open>We use three simple typing properties on integer values: 
+   is_IntVal32, is_IntVal64 and the more general is_IntVal.\<close>
+
+definition is_IntVal :: "Value \<Rightarrow> bool" where
+  "is_IntVal v = (is_IntVal32 v \<or> is_IntVal64 v)"
+
+lemma unary_eval_int:
+  assumes def: "unary_eval op x \<noteq> UndefVal"
+  shows "is_IntVal (unary_eval op x)"
+  apply (cases op; cases x)
+  unfolding is_IntVal_def using def by auto
+
+lemma bin_eval_int:
+  assumes def: "bin_eval op x y \<noteq> UndefVal"
+  shows "is_IntVal (bin_eval op x y)"
+  apply (cases op; cases x; cases y)  (* 300 cases! *)
+  unfolding is_IntVal_def using def apply auto (* prove the 294 easy cases *)
+  by (metis (full_types) bool_to_val.simps is_IntVal32_def)+
+
+lemma int_stamp32:
+  assumes i: "is_IntVal32 v"
+  shows "is_IntegerStamp (constantAsStamp v)"
+  using i unfolding is_IntegerStamp_def is_IntVal32_def by auto
+
+lemma int_stamp64:
+  assumes i: "is_IntVal64 v"
+  shows "is_IntegerStamp (constantAsStamp v)"
+  using i unfolding is_IntegerStamp_def is_IntVal64_def by auto
+
+lemma int_stamp_both:
+  assumes i: "is_IntVal v"
+  shows "is_IntegerStamp (constantAsStamp v)"
+  using i unfolding is_IntVal_def is_IntegerStamp_def
+  using int_stamp32 int_stamp64 is_IntegerStamp_def by auto 
+
+lemma validDefIntConst:
+  assumes "v \<noteq> UndefVal"
+  assumes "is_IntegerStamp (constantAsStamp v)"
+  shows "valid_value v (constantAsStamp v)"
+  using assms by (cases v; auto)
+
+lemma validIntConst:
+  assumes i: "is_IntVal v"
+  shows "valid_value v (constantAsStamp v)"
+  using i int_stamp_both is_IntVal_def validDefIntConst by auto 
+
+
+section \<open>Optimizations for Add Nodes\<close>
 
 phase SnipPhase 
   terminating size
@@ -9,16 +61,86 @@ begin
 
 optimization BinaryFoldConstant: "BinaryExpr op (const v1) (const v2) \<mapsto> ConstantExpr (bin_eval op v1 v2)"
    apply unfold_optimization
-  sorry
+   defer apply (cases op; simp)
+  unfolding le_expr_def
+  apply (rule allI impI)+
+  subgoal premises bin for m p v
+    print_facts
+    apply (rule BinaryExprE[OF bin])
+    subgoal premises prems for x y
+      print_facts
+(* backward refinement:
+      apply (subgoal_tac "x = v1 \<and> y = v2")
+        using prems apply auto
+      apply (rule ConstantExpr)
+      apply (rule validIntConst)
+      using bin_eval_int int_stamp_both by auto
+*)
+(* or forward proof: *)
+    proof -
+      have x: "x = v1" using prems by auto
+      have y: "y = v2" using prems by auto
+      have xy: "v = bin_eval op x y" using prems x y by simp
+      have int: "is_IntVal v" using bin_eval_int prems by auto
+      show ?thesis
+        unfolding prems x y xy (* get it in form: ConstantExpr c \<mapsto> c *)
+        apply (rule ConstantExpr)
+        apply (rule validIntConst)
+        using prems x y xy int by auto+
+      qed
+    done
+  done
+
 
 thm BinaryFoldConstant(1)
 thm BinaryFoldConstant(2)
 thm BinaryFoldConstant
 value "BinaryFoldConstant_code (ConstantExpr (IntVal32 0))"
 
+lemma size_pos[simp]: "0 < size y"
+  apply (induction y; auto?)
+  subgoal premises prems for op a b
+    using prems by (induction op; auto)
+  done
+
+lemma size_non_add: "op \<noteq> BinAdd \<Longrightarrow> size (BinaryExpr op a b) = size a + size b"
+  by (induction op; auto)
+
+lemma size_non_const:
+  "\<not> is_ConstantExpr y \<Longrightarrow> 1 < size y"
+  using size_pos apply (induction y; auto)
+  subgoal premises prems for op a b
+    apply (cases "op = BinAdd")
+    using size_non_add size_pos apply auto
+    by (simp add: Suc_lessI one_is_add)+
+  done         
+
+lemma binadd_commute:
+  assumes "bin_eval BinAdd x y \<noteq> UndefVal"
+  shows "bin_eval BinAdd x y = bin_eval BinAdd y x"
+  using assms intval_add_sym by simp
+
+
+(* horrible backward proof - needs improving *)
 optimization AddShiftConstantRight: "((const v) + y) \<mapsto> y + (const v) when \<not>(is_ConstantExpr y)"
   apply unfold_optimization
-  sorry
+   defer using size_non_const apply fastforce
+  print_facts
+  unfolding le_expr_def
+  apply (rule impI)
+  subgoal premises 1
+  apply (rule allI impI)+
+    subgoal premises 2 for m p va
+      apply (rule BinaryExprE[OF 2])  (* go forward from v+y *)
+      subgoal premises 3 for x ya
+        apply (rule BinaryExpr)       (* go backward from y+v *)
+        using 3 apply simp
+        using 3 apply simp
+        using 3 binadd_commute apply auto
+        done
+      done
+    done
+  done
 
 optimization AddNeutral: "(e + (const (IntVal32 0))) \<mapsto> e"
   apply unfold_optimization
